more initialisation

Weidenbach_Book/Watched_Literals_Initialisation.thy
@@ -5,16 +5,87 @@ begin
 subsection \<open>Initialise Data structure\<close>
 
 type_synonym 'v twl_st_init = \<open>'v twl_st  \<times> 'v clauses\<close>
+
+
+fun get_trail_init :: \<open>'v twl_st_init \<Rightarrow> ('v, 'v clause) ann_lit list\<close> where
+  \<open>get_trail_init ((M, _, _, _, _, _, _), _) = M\<close>
+
+fun get_conflict_init :: \<open>'v twl_st_init \<Rightarrow> 'v cconflict\<close> where
+  \<open>get_conflict_init ((_, _, _, D, _, _, _, _), _) = D\<close>
+
+fun literals_to_update_init :: \<open>'v twl_st_init \<Rightarrow> 'v clause\<close> where
+  \<open>literals_to_update_init ((_, _, _, _, _, _, _, Q), _) = Q\<close>
+
+fun clauses_to_update_init :: \<open>'v twl_st_init \<Rightarrow> ('v literal \<times> 'v twl_cls) multiset\<close> where
+  \<open>clauses_to_update_init ((_, _, _, _, _, _, WS, _), _) = WS\<close>
+
+fun other_clauses_init :: \<open>'v twl_st_init \<Rightarrow> 'v clauses\<close> where
+  \<open>other_clauses_init ((_, _, _, _, _, _, _), OC) = OC\<close>
+
+fun add_to_init_clauses :: \<open>'v clause_l \<Rightarrow> 'v twl_st_init \<Rightarrow> 'v twl_st_init\<close> where
+  \<open>add_to_init_clauses C ((M, N, U, D, NE, UE, WS, Q), OC) =
+      ((M, add_mset (twl_clause_of C) N, U, D, NE, UE, WS, Q), OC)\<close>
+
+fun add_to_unit_init_clauses :: \<open>'v clause \<Rightarrow> 'v twl_st_init \<Rightarrow> 'v twl_st_init\<close> where
+  \<open>add_to_unit_init_clauses C ((M, N, U, D, NE, UE, WS, Q), OC) =
+      ((M, N, U, D, add_mset C NE, UE, WS, Q), OC)\<close>
+
+fun set_conflict_init :: \<open>'v clause_l \<Rightarrow> 'v twl_st_init \<Rightarrow> 'v twl_st_init\<close> where
+ \<open>set_conflict_init C ((M, N, U, _, NE, UE, WS, Q), OC) =
+       ((M, N, U, Some (mset C), add_mset (mset C) NE, UE, {#}, {#}), OC)\<close>
+
+fun propagate_unit_init :: \<open>'v literal \<Rightarrow> 'v twl_st_init \<Rightarrow> 'v twl_st_init\<close> where
+ \<open>propagate_unit_init L ((M, N, U, D, NE, UE, WS, Q), OC) =
+       ((Propagated L {#L#} # M, N, U, D, add_mset {#L#} NE, UE, WS, add_mset (-L) Q), OC)\<close>
+
 type_synonym 'v twl_st_l_init = \<open>'v twl_st_l \<times> 'v clauses\<close>
+
+fun get_trail_l_init :: \<open>'v twl_st_l_init \<Rightarrow> ('v, nat) ann_lit list\<close> where
+  \<open>get_trail_l_init ((M, _, _, _, _, _, _), _) = M\<close>
+
+fun get_conflict_l_init :: \<open>'v twl_st_l_init \<Rightarrow> 'v cconflict\<close> where
+  \<open>get_conflict_l_init ((_, _, D, _, _, _, _), _) = D\<close>
+
+fun get_clauses_l_init :: \<open>'v twl_st_l_init \<Rightarrow> 'v clauses_l\<close> where
+  \<open>get_clauses_l_init ((M, N, D, NE, UE, WS, Q), _) = N\<close>
+
+fun literals_to_update_l_init :: \<open>'v twl_st_l_init \<Rightarrow> 'v clause\<close> where
+  \<open>literals_to_update_l_init ((_, _, _, _, _, _, Q), _) = Q\<close>
+
+fun clauses_to_update_l_init :: \<open>'v twl_st_l_init \<Rightarrow> 'v clauses_to_update_l\<close> where
+  \<open>clauses_to_update_l_init ((_, _, _, _, _, WS, _), _) = WS\<close>
+
+fun other_clauses_l_init :: \<open>'v twl_st_l_init \<Rightarrow> 'v clauses\<close> where
+  \<open>other_clauses_l_init ((_, _, _, _, _, _, _), OC) = OC\<close>
 
 fun state\<^sub>W_of_init :: "'v twl_st_init \<Rightarrow> 'v cdcl\<^sub>W_restart_mset" where
 "state\<^sub>W_of_init ((M, N, U, C, NE, UE, Q), OC) =
-  (M, clause `# N + NE + OC, clause `# U + UE,  C)"
+  (M, clause `# N + NE + OC, clause `# U + UE, C)"
 
-fun twl_st_of_init :: \<open>'v twl_st_l_init \<Rightarrow> 'v twl_st_init\<close> where
-  \<open>twl_st_of_init ((M, N, C, NE, UE, WS, Q), OC) =
-    ((convert_lits_l N M, twl_clause_of `# init_clss_lf N, twl_clause_of `# learned_clss_lf N,
-       C, NE, UE, {#}, Q), OC)\<close>
+
+named_theorems twl_st_init \<open>Convertion for inital theorems\<close>
+
+lemma [twl_st_init]:
+  \<open>get_conflict_init (S, QC) = get_conflict S\<close>
+  \<open>get_trail_init (S, QC) = get_trail S\<close>
+  \<open>clauses_to_update_init (S, QC) = clauses_to_update S\<close>
+  \<open>literals_to_update_init (S, QC) = literals_to_update S\<close>
+  by (solves \<open>cases S; auto\<close>)+
+
+
+definition twl_st_l_init :: \<open>('v twl_st_l_init \<times> 'v twl_st_init) set\<close> where
+  \<open>twl_st_l_init = {(((M, N, C, NE, UE, WS, Q), OC), ((M', N', C', NE', UE', WS', Q'), OC')).
+    ((M', N', C', NE', UE', WS', Q'), OC') =
+      ((convert_lits_l N M, twl_clause_of `# init_clss_lf N, twl_clause_of `# learned_clss_lf N,
+         C, NE, UE, {#}, Q), OC)}\<close>
+
+
+lemma [twl_st_init]:
+  assumes \<open>(S, T) \<in> twl_st_l_init\<close>
+  shows
+   \<open>get_trail_init T = convert_lits_l (get_clauses_l_init S) (get_trail_l_init S)\<close>
+   \<open>get_trail (fst T) = convert_lits_l (get_clauses_l_init S) (get_trail_l_init S)\<close>
+  by (use assms in \<open>solves \<open>cases S; auto simp: twl_st_l_init_def\<close>\<close>)+
 
 definition twl_struct_invs_init :: \<open>'v twl_st_init \<Rightarrow> bool\<close> where
   \<open>twl_struct_invs_init S \<longleftrightarrow>
@@ -27,7 +98,7 @@ definition twl_struct_invs_init :: \<open>'v twl_st_init \<Rightarrow> bool\<clo
     distinct_queued (fst S) \<and>
     confl_cands_enqueued (fst S) \<and>
     propa_cands_enqueued (fst S) \<and>
-    (get_conflict (fst S) \<noteq> None \<longrightarrow> clauses_to_update (fst S) = {#} \<and> literals_to_update (fst S) = {#}) \<and>
+    (get_conflict_init S \<noteq> None \<longrightarrow> clauses_to_update_init S = {#} \<and> literals_to_update_init S = {#}) \<and>
     entailed_clss_inv (fst S) \<and>
     clauses_to_update_inv (fst S) \<and>
     past_invs (fst S))
@@ -53,7 +124,7 @@ proof -
     to_upd: \<open>clauses_to_update_inv S\<close> and
     past: \<open>past_invs S\<close>
     using assms unfolding twl_struct_invs_init_def fst_conv
-    by clarify+
+    by (auto simp add: twl_st_init)
 
   show ?thesis
     unfolding twl_struct_invs_init_def fst_conv
@@ -75,36 +146,68 @@ proof -
     subgoal by (rule dist)
     subgoal by (rule cands_confl)
     subgoal by (rule cands_propa)
-    subgoal by (rule confl)
+    subgoal using confl by (auto simp: twl_st_init)
     subgoal by (rule unit)
     subgoal by (rule to_upd)
     subgoal by (rule past)
     done
 qed
 
+fun add_empty_conflict_init_l :: \<open>'v twl_st_l_init \<Rightarrow> 'v twl_st_l_init\<close> where
+  add_empty_conflict_init_def[simp del]:
+   \<open>add_empty_conflict_init_l ((M, N, D, NE, UE, WS, Q), OC) =
+       ((M, N, Some {#}, NE, UE, WS, Q), add_mset {#} OC)\<close>
+
+
+fun propagate_unit_init_l :: \<open>'v literal \<Rightarrow> 'v twl_st_l_init \<Rightarrow> 'v twl_st_l_init\<close> where
+  propagate_unit_init_l_def[simp del]:
+   \<open>propagate_unit_init_l L ((M, N, D, NE, UE, WS, Q), OC) =
+       ((Propagated L 0 # M, N, D, add_mset {#L#} NE, UE, WS, add_mset (-L) Q), OC)\<close>
+
+
+fun already_propagated_unit_init_l :: \<open>'v clause \<Rightarrow> 'v twl_st_l_init \<Rightarrow> 'v twl_st_l_init\<close> where
+  already_propagated_unit_init_l_def[simp del]:
+   \<open>already_propagated_unit_init_l C ((M, N, D, NE, UE, WS, Q), OC) =
+       ((M, N, D, add_mset C NE, UE, WS, Q), OC)\<close>
+
+
+fun set_conflict_init_l :: \<open>'v clause_l \<Rightarrow> 'v twl_st_l_init \<Rightarrow> 'v twl_st_l_init\<close> where
+  set_conflict_init_l_def[simp del]:
+   \<open>set_conflict_init_l C ((M, N, _, NE, UE, WS, Q), OC) =
+       ((M, N, Some (mset C), add_mset (mset C) NE, UE, {#}, {#}), OC)\<close>
+
+
+fun add_to_clauses_init_l :: \<open>'v clause_l \<Rightarrow> 'v twl_st_l_init \<Rightarrow> 'v twl_st_l_init nres\<close> where
+  add_to_clauses_init_l_def[simp del]:
+   \<open>add_to_clauses_init_l C ((M, N, _, NE, UE, WS, Q), OC) = do {
+        i \<leftarrow> get_fresh_index N;
+        RETURN ((M, fmupd i (C, True) N, None, NE, UE, WS, Q), OC)
+    }\<close>
+
+fun add_to_other_init where
+  \<open>add_to_other_init C (S, OC) = (S, add_mset (mset C) OC)\<close>
+
+lemma fst_add_to_other_init [simp]: \<open>fst (add_to_other_init a T) = fst T\<close>
+  by (cases T) auto
+
 definition init_dt_step :: \<open>'v clause_l \<Rightarrow> 'v twl_st_l_init \<Rightarrow> 'v twl_st_l_init nres\<close> where
   \<open>init_dt_step C S =
-  (let ((M, N, D, NE, UE, WS, Q), OC) = S in
-  (case D of
+  (case get_conflict_l (fst S) of
     None \<Rightarrow>
     if length C = 0
-    then RETURN ((M, N, Some {#}, NE, UE, {#}, {#}), add_mset {#} OC)
+    then RETURN (add_empty_conflict_init_l S)
     else if length C = 1
     then
       let L = hd C in
-      if undefined_lit M L
-      then RETURN ((Propagated L 0 # M, N, None, add_mset {#L#} NE, UE, WS, add_mset (-L) Q), OC)
-      else if L \<in> lits_of_l M
-      then RETURN ((M, N, None, add_mset {#L#} NE, UE, WS, Q), OC)
-      else RETURN ((M, N, Some (mset C), add_mset {#L#} NE, UE, {#}, {#}), OC)
+      if undefined_lit (get_trail_l_init S) L
+      then RETURN (propagate_unit_init_l L S)
+      else if L \<in> lits_of_l (get_trail_l_init S)
+      then RETURN (already_propagated_unit_init_l (mset C) S)
+      else RETURN (set_conflict_init_l C S)
     else
-      let L = hd C; L' = hd (tl C); C' = tl (tl C) in
-      do {
-        i \<leftarrow> get_fresh_index N;
-        RETURN ((M, fmupd i ([L, L'] @ C', True) N, None, NE, UE, WS, Q), OC)
-      }
+        add_to_clauses_init_l C S
   | Some D \<Rightarrow>
-      RETURN ((M, N, Some D, NE, UE, WS, Q), add_mset (mset C) OC)))\<close>
+      RETURN (add_to_other_init C S))\<close>
 
 fun init_dt :: \<open>'v clause_l list \<Rightarrow> 'v twl_st_l_init \<Rightarrow> 'v twl_st_l_init nres\<close> where
   \<open>init_dt [] S = RETURN S\<close>
@@ -113,23 +216,1003 @@ fun init_dt :: \<open>'v clause_l list \<Rightarrow> 'v twl_st_l_init \<Rightarr
       init_dt CS S
    }\<close>
 
-lemma init_dt_full:
-  fixes CS :: \<open>'v literal list list\<close> and S :: \<open>'v twl_st_l\<close> and OC :: \<open>'v clauses\<close>
-  defines \<open>SOC' \<equiv> init_dt CS (S, OC)\<close>
-  defines \<open>S' \<equiv> fst (init_dt CS (S, OC))\<close>
-  defines \<open>OC' \<equiv> snd (init_dt CS (S, OC))\<close>
-  assumes
-    \<open>\<forall>C \<in> set CS. distinct C\<close> and
-    \<open>twl_struct_invs_init (twl_st_of_init (S, OC))\<close> and
-    \<open>clauses_to_update_l S = {#}\<close> and
-    \<open>\<forall>s\<in>set (get_trail_l S). \<not>is_decided s\<close> and
-    \<open>get_conflict_l S = None \<longrightarrow> literals_to_update_l S = uminus `# lit_of `# mset (get_trail_l S)\<close> and
-    \<open>twl_list_invs S\<close> and
-    \<open>get_learned_l S = length (get_clauses_l S) - 1\<close> and
-    \<open>twl_stgy_invs (twl_st_of None S)\<close> and
-    \<open>OC \<noteq> {#} \<longrightarrow> get_conflict_l S \<noteq> None\<close>
+definition   init_dt_pre where
+  \<open>init_dt_pre CS SOC \<longleftrightarrow>
+    (\<exists>T. (SOC, T) \<in> twl_st_l_init \<and>
+      (\<forall>C \<in> set CS. distinct C) \<and>
+      twl_struct_invs_init T \<and>
+      clauses_to_update_l_init SOC = {#} \<and>
+      (\<forall>s\<in>set (get_trail_l_init SOC). \<not>is_decided s) \<and>
+      (get_conflict_l_init SOC = None \<longrightarrow>
+          literals_to_update_l_init SOC = uminus `# lit_of `# mset (get_trail_l_init SOC)) \<and>
+      twl_list_invs (fst SOC) \<and>
+      twl_stgy_invs (fst T) \<and>
+      (other_clauses_l_init SOC \<noteq> {#} \<longrightarrow> get_conflict_l_init SOC \<noteq> None))\<close>
+
+lemma init_dt_pre_ConsD: \<open>init_dt_pre (a # CS) SOC \<Longrightarrow> init_dt_pre CS SOC \<and> distinct a\<close>
+  unfolding init_dt_pre_def
+  apply normalize_goal+
+  by fastforce
+
+definition init_dt_spec where
+  \<open>init_dt_spec CS SOC = (\<lambda>(S', OC'). 
+       \<exists>T'. ((S', OC'), T') \<in> twl_st_l_init \<and>
+           twl_struct_invs_init T' \<and>
+           clauses_to_update_l S' = {#} \<and>
+           (\<forall>s\<in>set (get_trail_l S'). \<not>is_decided s) \<and>
+           (get_conflict_l S' = None \<longrightarrow>
+              literals_to_update_l S' = uminus `# lit_of `# mset (get_trail_l S')) \<and>
+           (mset `# mset CS + mset `# ran_mf (get_clauses_l (fst SOC)) + snd SOC =
+              mset `# ran_mf (get_clauses_l S') + OC') \<and>
+           learned_clss_lf (get_clauses_l (fst SOC)) = learned_clss_lf (get_clauses_l S') \<and>
+           twl_list_invs S' \<and>
+           twl_stgy_invs (fst T') \<and>
+           (OC' \<noteq> {#} \<longrightarrow> get_conflict_l S' \<noteq> None) \<and>
+           ({#} \<in># mset `# mset CS \<longrightarrow> get_conflict_l S' \<noteq> None))\<close>
+
+
+lemma twl_struct_invs_init_add_to_other_init:
+  assumes 
+    dist: \<open>distinct a\<close> and
+    lev: \<open>count_decided (get_trail (fst T)) = 0\<close> and
+    invs: \<open>twl_struct_invs_init T\<close>
   shows
-    \<open>twl_struct_invs_init (twl_st_of_init SOC')\<close> and
+    \<open>twl_struct_invs_init (add_to_other_init a T)\<close>
+      (is ?twl_struct_invs_init)
+proof -
+  obtain M N U D NE UE Q OC WS where
+    T: \<open>T = ((M, N, U, D, NE, UE, WS, Q), OC)\<close>
+    by (cases T) auto
+  have \<open>cdcl\<^sub>W_restart_mset.cdcl\<^sub>W_all_struct_inv (M, clauses N + NE + OC, clauses U + UE, D)\<close>
+    using invs unfolding T twl_struct_invs_init_def by auto
+  then have [simp]: 
+   \<open>cdcl\<^sub>W_restart_mset.cdcl\<^sub>W_all_struct_inv (M, add_mset (mset a) (clauses N + NE + OC), clauses U + UE, D)\<close>
+    using dist
+    by (auto simp: cdcl\<^sub>W_restart_mset.cdcl\<^sub>W_all_struct_inv_def
+       cdcl\<^sub>W_restart_mset.no_strange_atm_def cdcl\<^sub>W_restart_mset_state
+       cdcl\<^sub>W_restart_mset.cdcl\<^sub>W_M_level_inv_def cdcl\<^sub>W_restart_mset.cdcl\<^sub>W_conflicting_def
+        cdcl\<^sub>W_restart_mset.distinct_cdcl\<^sub>W_state_def all_decomposition_implies_def
+        clauses_def cdcl\<^sub>W_restart_mset.cdcl\<^sub>W_learned_clause_def)
+
+  have \<open>cdcl\<^sub>W_restart_mset.no_smaller_propa (M, clauses N + NE + OC, clauses U + UE, D)\<close>
+    using invs unfolding T twl_struct_invs_init_def by auto
+  then have [simp]:
+     \<open>cdcl\<^sub>W_restart_mset.no_smaller_propa (M, add_mset (mset a) (clauses N + NE + OC),
+        clauses U + UE, D)\<close>
+    using lev
+    by (auto simp: cdcl\<^sub>W_restart_mset.no_smaller_propa_def cdcl\<^sub>W_restart_mset_state
+        clauses_def T count_decided_0_iff)
+  show ?twl_struct_invs_init
+    using invs
+    unfolding twl_struct_invs_init_def T
+    unfolding fst_conv add_to_other_init.simps state\<^sub>W_of_init.simps get_conflict.simps
+    by clarsimp
+qed
+
+
+lemma twl_struct_invs_init_add_to_unit_init_clauses:
+  assumes 
+    dist: \<open>distinct a\<close> and
+    lev: \<open>count_decided (get_trail (fst T)) = 0\<close> and
+    invs: \<open>twl_struct_invs_init T\<close> and
+    ex: \<open>\<exists>L \<in> set a. L \<in> lits_of_l (get_trail_init T)\<close>
+  shows
+    \<open>twl_struct_invs_init (add_to_unit_init_clauses (mset a) T)\<close>
+      (is ?all_struct)
+proof -
+  obtain M N U D NE UE Q OC WS where
+    T: \<open>T = ((M, N, U, D, NE, UE, WS, Q), OC)\<close>
+    by (cases T) auto
+  have \<open>cdcl\<^sub>W_restart_mset.cdcl\<^sub>W_all_struct_inv (M, clauses N + NE + OC, clauses U + UE, D)\<close>
+    using invs unfolding T twl_struct_invs_init_def by auto
+  then have [simp]: 
+   \<open>cdcl\<^sub>W_restart_mset.cdcl\<^sub>W_all_struct_inv (M, add_mset (mset a) (clauses N + NE + OC), clauses U + UE, D)\<close>
+    using twl_struct_invs_init_add_to_other_init[OF dist lev invs]
+    unfolding T twl_struct_invs_init_def
+    by simp
+
+  have \<open>cdcl\<^sub>W_restart_mset.no_smaller_propa (M, clauses N + NE + OC, clauses U + UE, D)\<close>
+    using invs unfolding T twl_struct_invs_init_def by auto
+  then have [simp]:
+     \<open>cdcl\<^sub>W_restart_mset.no_smaller_propa (M, add_mset (mset a) (clauses N + NE + OC),
+        clauses U + UE, D)\<close>
+    using lev
+    by (auto simp: cdcl\<^sub>W_restart_mset.no_smaller_propa_def cdcl\<^sub>W_restart_mset_state
+        clauses_def T count_decided_0_iff)
+  have [simp]: \<open>confl_cands_enqueued (M, N, U, D, add_mset (mset a) NE, UE, WS, Q) \<longleftrightarrow>
+     confl_cands_enqueued (M, N, U, D, NE, UE, WS, Q)\<close>
+    \<open>propa_cands_enqueued (M, N, U, D, add_mset (mset a) NE, UE, WS, Q) \<longleftrightarrow>
+      propa_cands_enqueued (M, N, U, D, NE, UE, WS, Q)\<close>
+    \<open>twl_st_inv (M, N, U, D, add_mset (mset a) NE, UE, WS, Q) \<longleftrightarrow>
+        twl_st_inv (M, N, U, D, NE, UE, WS, Q)\<close>
+    \<open>\<And>x.  twl_exception_inv (M, N, U, D, add_mset (mset a) NE, UE, WS, Q) x \<longleftrightarrow>
+          twl_exception_inv (M, N, U, D, NE, UE, WS, Q) x\<close>
+    \<open>clauses_to_update_inv (M, N, U, D, add_mset (mset a) NE, UE, WS, Q) \<longleftrightarrow>
+       clauses_to_update_inv (M, N, U, D, NE, UE, WS, Q)\<close>
+    \<open>past_invs (M, N, U, D, add_mset (mset a) NE, UE, WS, Q) \<longleftrightarrow>
+        past_invs (M, N, U, D, NE, UE, WS, Q)\<close>
+    by (cases D; auto simp: twl_st_inv.simps twl_exception_inv.simps past_invs.simps; fail)+
+  have [simp]: \<open>entailed_clss_inv (M, N, U, D, add_mset (mset a) NE, UE, WS, Q) \<longleftrightarrow>
+     entailed_clss_inv (M, N, U, D, NE, UE, WS, Q)\<close>
+    using ex count_decided_ge_get_level[of M] lev by (cases D) (auto simp: T)
+  show ?all_struct
+    using invs ex
+    unfolding twl_struct_invs_init_def T
+    unfolding fst_conv add_to_other_init.simps state\<^sub>W_of_init.simps get_conflict.simps
+    by (clarsimp simp del: entailed_clss_inv.simps)
+qed
+
+lemma twl_struct_invs_init_set_conflict_init:
+  assumes 
+    dist: \<open>distinct C\<close> and
+    lev: \<open>count_decided (get_trail (fst T)) = 0\<close> and
+    invs: \<open>twl_struct_invs_init T\<close> and
+    ex: \<open>\<forall>L \<in> set C. -L \<in> lits_of_l (get_trail_init T)\<close> and
+    nempty: \<open>C \<noteq> []\<close>
+  shows
+    \<open>twl_struct_invs_init (set_conflict_init C T)\<close>
+      (is ?all_struct)
+proof -
+  obtain M N U D NE UE Q OC WS where
+    T: \<open>T = ((M, N, U, D, NE, UE, WS, Q), OC)\<close>
+    by (cases T) auto
+  have \<open>cdcl\<^sub>W_restart_mset.cdcl\<^sub>W_all_struct_inv (M, clauses N + NE + OC, clauses U + UE, D)\<close>
+    using invs unfolding T twl_struct_invs_init_def by auto
+  then have [simp]: 
+   \<open>cdcl\<^sub>W_restart_mset.cdcl\<^sub>W_all_struct_inv (M, add_mset (mset C) (clauses N + NE + OC),
+        clauses U + UE, Some (mset C))\<close>
+    using dist ex
+    unfolding T twl_struct_invs_init_def
+    by (auto 5 5 simp: cdcl\<^sub>W_restart_mset.cdcl\<^sub>W_all_struct_inv_def
+       cdcl\<^sub>W_restart_mset.no_strange_atm_def cdcl\<^sub>W_restart_mset_state
+       cdcl\<^sub>W_restart_mset.cdcl\<^sub>W_M_level_inv_def cdcl\<^sub>W_restart_mset.cdcl\<^sub>W_conflicting_def
+       cdcl\<^sub>W_restart_mset.distinct_cdcl\<^sub>W_state_def all_decomposition_implies_def
+       clauses_def cdcl\<^sub>W_restart_mset.cdcl\<^sub>W_learned_clause_def
+       true_annots_true_cls_def_iff_negation_in_model)
+
+  have \<open>cdcl\<^sub>W_restart_mset.no_smaller_propa (M, clauses N + NE + OC, clauses U + UE, D)\<close>
+    using invs unfolding T twl_struct_invs_init_def by auto
+  then have [simp]:
+     \<open>cdcl\<^sub>W_restart_mset.no_smaller_propa (M, add_mset (mset C) (clauses N + NE + OC),
+        clauses U + UE, Some (mset C))\<close>
+    using lev
+    by (auto simp: cdcl\<^sub>W_restart_mset.no_smaller_propa_def cdcl\<^sub>W_restart_mset_state
+        clauses_def T count_decided_0_iff)
+  let ?T = \<open>(M, N, U, Some (mset C), add_mset (mset C) NE, UE, {#}, {#})\<close>
+  have [simp]: \<open>confl_cands_enqueued ?T\<close>
+    \<open>propa_cands_enqueued ?T\<close>
+    \<open>twl_st_inv (M, N, U, D, NE, UE, WS, Q) \<Longrightarrow> twl_st_inv ?T\<close>
+    \<open>\<And>x.  twl_exception_inv (M, N, U, D, NE, UE, WS, Q) x \<Longrightarrow> twl_exception_inv ?T x\<close>
+    \<open>clauses_to_update_inv (M, N, U, D, NE, UE, WS, Q) \<Longrightarrow> clauses_to_update_inv ?T\<close>
+    \<open>past_invs (M, N, U, D, NE, UE, WS, Q) \<Longrightarrow> past_invs ?T\<close>
+    by (auto simp: twl_st_inv.simps twl_exception_inv.simps past_invs.simps; fail)+
+  have [simp]: \<open> entailed_clss_inv (M, N, U, D, NE, UE, WS, Q) \<Longrightarrow> entailed_clss_inv ?T\<close>
+    using ex count_decided_ge_get_level[of M] lev nempty by (auto simp: T)
+  show ?all_struct
+    using invs ex
+    unfolding twl_struct_invs_init_def T
+    unfolding fst_conv add_to_other_init.simps state\<^sub>W_of_init.simps get_conflict.simps
+    by (clarsimp simp del: entailed_clss_inv.simps)
+qed
+
+lemma twl_struct_invs_init_propagate_unit_init:
+  assumes
+    lev: \<open>count_decided (get_trail (fst T)) = 0\<close> and
+    invs: \<open>twl_struct_invs_init T\<close> and
+    undef: \<open>undefined_lit (get_trail_init T) L\<close>
+  shows
+    \<open>twl_struct_invs_init (propagate_unit_init L T)\<close>
+      (is ?all_struct)
+proof -
+  obtain M N U D NE UE Q OC WS where
+    T: \<open>T = ((M, N, U, D, NE, UE, WS, Q), OC)\<close>
+    by (cases T) auto
+  have [iff]: \<open>- L \<in> lits_of_l M \<longleftrightarrow> False\<close>
+    using undef by (auto simp: T Decided_Propagated_in_iff_in_lits_of_l)
+  have [simp]: \<open>get_all_ann_decomposition M = [([], M)]\<close>
+    by (rule no_decision_get_all_ann_decomposition) (use lev in \<open>auto simp: T count_decided_0_iff\<close>)
+  have H: \<open>a @ Propagated L' mark' # b = Propagated L mark # M  \<longleftrightarrow>
+     (a = [] \<and> L = L' \<and> mark = mark' \<and> b = M) \<or>
+     (a \<noteq> [] \<and> hd a = Propagated L mark \<and> tl a @ Propagated L' mark' # b = M)\<close>
+    for a mark mark' L' b
+    using undef by (cases a) (auto simp: T atm_of_eq_atm_of)
+  have \<open>cdcl\<^sub>W_restart_mset.cdcl\<^sub>W_all_struct_inv (M, clauses N + NE + OC, clauses U + UE, D)\<close>
+    using invs unfolding T twl_struct_invs_init_def by auto
+  then have [simp]: 
+   \<open>cdcl\<^sub>W_restart_mset.cdcl\<^sub>W_all_struct_inv (M, add_mset {#L#} (clauses N + NE + OC), clauses U + UE, D)\<close>
+    by (auto simp: cdcl\<^sub>W_restart_mset.cdcl\<^sub>W_all_struct_inv_def
+       cdcl\<^sub>W_restart_mset.no_strange_atm_def cdcl\<^sub>W_restart_mset_state
+       cdcl\<^sub>W_restart_mset.cdcl\<^sub>W_M_level_inv_def cdcl\<^sub>W_restart_mset.cdcl\<^sub>W_conflicting_def
+        cdcl\<^sub>W_restart_mset.distinct_cdcl\<^sub>W_state_def all_decomposition_implies_def
+        clauses_def cdcl\<^sub>W_restart_mset.cdcl\<^sub>W_learned_clause_def)
+  then have [simp]: 
+   \<open>cdcl\<^sub>W_restart_mset.cdcl\<^sub>W_all_struct_inv (Propagated L {#L#} # M,
+        add_mset {#L#} (clauses N + NE + OC), clauses U + UE, D)\<close>
+    using undef by (auto simp: cdcl\<^sub>W_restart_mset.cdcl\<^sub>W_all_struct_inv_def T H
+       cdcl\<^sub>W_restart_mset.no_strange_atm_def cdcl\<^sub>W_restart_mset_state
+       cdcl\<^sub>W_restart_mset.cdcl\<^sub>W_M_level_inv_def cdcl\<^sub>W_restart_mset.cdcl\<^sub>W_conflicting_def
+        cdcl\<^sub>W_restart_mset.distinct_cdcl\<^sub>W_state_def all_decomposition_implies_def
+        clauses_def cdcl\<^sub>W_restart_mset.cdcl\<^sub>W_learned_clause_def
+        consistent_interp_insert_iff)
+  have [iff]: \<open>Propagated L {#L#} # M = M' @ Decided K # Ma \<longleftrightarrow> False\<close> for M' K Ma
+    sorry
+  have \<open>cdcl\<^sub>W_restart_mset.no_smaller_propa (M, clauses N + NE + OC, clauses U + UE, D)\<close>
+    using invs unfolding T twl_struct_invs_init_def by auto
+  then have [simp]:
+     \<open>cdcl\<^sub>W_restart_mset.no_smaller_propa (Propagated L {#L#} # M, add_mset {#L#} (clauses N + NE + OC),
+        clauses U + UE, D)\<close>
+    using lev
+    by (auto simp: cdcl\<^sub>W_restart_mset.no_smaller_propa_def cdcl\<^sub>W_restart_mset_state
+        clauses_def T count_decided_0_iff)
+
+  have \<open>cdcl\<^sub>W_restart_mset.no_smaller_propa (M, clauses N + NE + OC, clauses U + UE, D)\<close>
+    using invs unfolding T twl_struct_invs_init_def by auto
+  then have [simp]:
+     \<open>cdcl\<^sub>W_restart_mset.no_smaller_propa (Propagated L {#L#} # M, add_mset {#L#} (clauses N + NE + OC),
+        clauses U + UE, D)\<close>
+    using lev
+    by (auto simp: cdcl\<^sub>W_restart_mset.no_smaller_propa_def cdcl\<^sub>W_restart_mset_state
+        clauses_def T count_decided_0_iff)
+  let ?T = \<open>(Propagated L {#L#} # M, N, U, D, add_mset {#L#} NE, UE, WS, add_mset (-L) Q)\<close>
+  have [simp]:
+     \<open>confl_cands_enqueued (M, N, U, D, NE, UE, WS, Q) \<Longrightarrow>
+       confl_cands_enqueued ?T\<close>
+    \<open>propa_cands_enqueued (M, N, U, D, NE, UE, WS, Q) \<Longrightarrow>propa_cands_enqueued ?T\<close>
+    \<open>twl_st_inv (M, N, U, D, NE, UE, WS, Q) \<Longrightarrow> twl_st_inv ?T\<close>
+    \<open>\<And>x.  twl_exception_inv (M, N, U, D, NE, UE, WS, Q) x \<Longrightarrow> twl_exception_inv ?T x\<close>
+    \<open>clauses_to_update_inv (M, N, U, D, NE, UE, WS, Q) \<Longrightarrow> clauses_to_update_inv ?T\<close>
+    \<open>past_invs (M, N, U, D, NE, UE, WS, Q) \<Longrightarrow> past_invs ?T\<close>
+         apply (cases D; auto simp: twl_st_inv.simps twl_exception_inv.simps past_invs.simps)
+    sorry
+  have [simp]: \<open>entailed_clss_inv (M, N, U, D, NE, UE, WS, Q) \<Longrightarrow> entailed_clss_inv ?T\<close>
+    using ex count_decided_ge_get_level[of M] lev by (cases D) (auto simp: T get_level_cons_if)
+  show ?all_struct
+    using invs ex
+    unfolding twl_struct_invs_init_def T
+    unfolding fst_conv add_to_other_init.simps state\<^sub>W_of_init.simps get_conflict.simps
+    by (clarsimp simp del: entailed_clss_inv.simps clauses_to_update_inv.simps
+        valid_enqueued_alt_simps)
+qed
+
+named_theorems twl_st_l_init
+lemma [twl_st_l_init]:
+  \<open>clauses_to_update_l_init (already_propagated_unit_init_l C S) = clauses_to_update_l_init S\<close>
+  \<open>get_trail_l_init (already_propagated_unit_init_l C S) = get_trail_l_init S\<close>
+  \<open>get_conflict_l_init (already_propagated_unit_init_l C S) = get_conflict_l_init S\<close>
+  \<open>other_clauses_l_init (already_propagated_unit_init_l C S) = other_clauses_l_init S\<close>
+  \<open>clauses_to_update_l_init (already_propagated_unit_init_l C S) = clauses_to_update_l_init S\<close>
+  \<open>literals_to_update_l_init (already_propagated_unit_init_l C S) = literals_to_update_l_init S\<close>
+  \<open>get_conflict_l_init (T, OC) = get_conflict_l T\<close>
+  by (solves \<open>cases S; cases T; auto simp: already_propagated_unit_init_l_def\<close>)+
+
+lemma [twl_st_init]:
+  \<open>clauses_to_update_init (add_to_unit_init_clauses (mset C) T) = clauses_to_update_init T\<close>
+  \<open>literals_to_update_init (add_to_unit_init_clauses (mset C) T) = literals_to_update_init T\<close>
+  \<open>get_conflict_init (add_to_unit_init_clauses (mset C) T) = get_conflict_init T\<close>
+  apply (cases T; auto simp: twl_st_inv.simps; fail)+
+  done
+
+lemma [twl_st_init]:
+  \<open>twl_st_inv (fst (add_to_unit_init_clauses (mset C) T)) \<longleftrightarrow>  twl_st_inv (fst T)\<close>
+  \<open>valid_enqueued (fst (add_to_unit_init_clauses (mset C) T)) \<longleftrightarrow> valid_enqueued (fst T)\<close>
+  \<open>no_duplicate_queued (fst (add_to_unit_init_clauses (mset C) T)) \<longleftrightarrow> no_duplicate_queued (fst T)\<close>
+  \<open>distinct_queued (fst (add_to_unit_init_clauses (mset C) T)) \<longleftrightarrow> distinct_queued (fst T)\<close>
+  \<open>confl_cands_enqueued (fst (add_to_unit_init_clauses (mset C) T)) \<longleftrightarrow> confl_cands_enqueued (fst T)\<close>
+  \<open>propa_cands_enqueued (fst (add_to_unit_init_clauses (mset C) T)) \<longleftrightarrow> propa_cands_enqueued (fst T)\<close>
+  \<open>twl_st_exception_inv (fst (add_to_unit_init_clauses (mset C) T)) \<longleftrightarrow> twl_st_exception_inv (fst T)\<close>
+    apply (cases T; auto simp: twl_st_inv.simps; fail)+
+  apply (cases \<open>get_conflict_init T\<close>; cases T;
+      auto simp: twl_st_inv.simps twl_exception_inv.simps; fail)+
+  done
+
+lemma entailed_clss_inv_add_to_unit_init_clauses:
+  \<open>count_decided (get_trail_init T) = 0 \<Longrightarrow> C \<noteq> [] \<Longrightarrow> hd C \<in> lits_of_l (get_trail_init T) \<Longrightarrow>
+     entailed_clss_inv (fst T) \<Longrightarrow> entailed_clss_inv (fst (add_to_unit_init_clauses (mset C) T))\<close>
+  using count_decided_ge_get_level[of \<open>get_trail_init T\<close>]
+  by (cases T; cases C; auto simp: twl_st_inv.simps twl_exception_inv.simps)
+
+lemma init_dt_pre_already_propagated_unit_init_l:
+  assumes 
+    hd_C: \<open>hd C \<in> lits_of_l (get_trail_l_init S)\<close> and
+    pre: \<open>init_dt_pre CS S\<close> and
+    nempty: \<open>C \<noteq> []\<close> and
+    dist_C: \<open>distinct C\<close> and
+    lev: \<open>count_decided (get_trail_l_init S) = 0\<close>
+  shows \<open>init_dt_pre CS (already_propagated_unit_init_l (mset C) S)\<close>
+proof -
+  obtain T where
+    SOC_T: \<open>(S, T) \<in> twl_st_l_init\<close> and
+    dist: \<open>Ball (set CS) distinct\<close> and
+    inv: \<open>twl_struct_invs_init T\<close> and
+    WS: \<open>clauses_to_update_l_init S = {#}\<close> and
+    dec: \<open>\<forall>s\<in>set (get_trail_l_init S). \<not> is_decided s\<close> and
+    in_literals_to_update: \<open>get_conflict_l_init S = None \<longrightarrow>
+     literals_to_update_l_init S = uminus `# lit_of `# mset (get_trail_l_init S)\<close> and
+    add_inv: \<open>twl_list_invs (fst S)\<close> and
+    stgy_inv: \<open>twl_stgy_invs (fst T)\<close> and
+    OC'_empty: \<open>other_clauses_l_init S \<noteq> {#} \<longrightarrow> get_conflict_l_init S \<noteq> None\<close>
+    using pre unfolding init_dt_pre_def
+    apply -
+    apply normalize_goal+
+    by presburger
+  obtain M N D NE UE Q U OC where
+    S: \<open>S = ((M, N, U, D, NE, UE, Q), OC)\<close>
+    by (cases S) auto
+  have [simp]: \<open>twl_list_invs (fst (already_propagated_unit_init_l (mset C) S))\<close>
+    using add_inv by (auto simp:  already_propagated_unit_init_l_def S
+        twl_list_invs_def)
+  have [simp]: \<open>(already_propagated_unit_init_l (mset C) S, add_to_unit_init_clauses (mset C) T)
+        \<in> twl_st_l_init\<close>
+    using SOC_T by (cases S) (auto simp: twl_st_l_init_def already_propagated_unit_init_l_def)
+  have dec': \<open>\<forall>s\<in>set (get_trail_init T). \<not> is_decided s\<close>
+    using SOC_T dec by (auto simp: twl_st_l_init twl_st_init convert_lits_l_def)
+  have [simp]: \<open>twl_stgy_invs (fst (add_to_unit_init_clauses (mset C) T))\<close>
+    using stgy_inv dec' unfolding twl_stgy_invs_def cdcl\<^sub>W_restart_mset.cdcl\<^sub>W_stgy_invariant_def
+       cdcl\<^sub>W_restart_mset.conflict_non_zero_unless_level_0_def cdcl\<^sub>W_restart_mset.no_smaller_confl_def
+    by (cases T)
+       (auto simp: cdcl\<^sub>W_restart_mset_state clauses_def)
+  note clauses_to_update_inv.simps[simp del] valid_enqueued_alt_simps[simp del]
+  have [simp]: \<open>twl_struct_invs_init (add_to_unit_init_clauses (mset C) T)\<close>
+    apply (rule twl_struct_invs_init_add_to_unit_init_clauses)
+    using inv hd_C nempty dist_C lev SOC_T dec
+    by (auto simp: twl_st_init count_decided_0_iff)
+  show ?thesis
+    unfolding init_dt_pre_def
+    apply (rule exI[of _ \<open>add_to_unit_init_clauses (mset C) T\<close>])
+    using dist WS dec in_literals_to_update OC'_empty by (auto simp: twl_st_init twl_st_l_init)
+qed
+
+lemma [twl_st_l_init]:
+  \<open>get_trail_l_init (set_conflict_init_l C S) = get_trail_l_init S\<close>
+  \<open>literals_to_update_l_init (set_conflict_init_l C S) = {#}\<close>
+  \<open>clauses_to_update_l_init (set_conflict_init_l C S) = {#}\<close>
+  \<open>get_conflict_l_init (set_conflict_init_l C S) = Some (mset C)\<close>
+  by (cases S; auto simp: set_conflict_init_l_def)+
+
+lemma init_dt_pre_set_conflict_init_l:
+  assumes 
+    \<open>get_conflict_l_init S = None\<close> and
+    pre: \<open>init_dt_pre (C # CS) S\<close> and
+    false: \<open>\<forall>L \<in> set C.  -L \<in> lits_of_l (get_trail_l_init S)\<close> and
+    nempty: \<open>C \<noteq> []\<close>
+  shows \<open>init_dt_pre CS (set_conflict_init_l C S)\<close>
+proof -
+  obtain T where
+    SOC_T: \<open>(S, T) \<in> twl_st_l_init\<close> and
+    dist: \<open>Ball (set CS) distinct\<close> and
+    dist_C: \<open>distinct C\<close> and
+    inv: \<open>twl_struct_invs_init T\<close> and
+    WS: \<open>clauses_to_update_l_init S = {#}\<close> and
+    dec: \<open>\<forall>s\<in>set (get_trail_l_init S). \<not> is_decided s\<close> and
+    in_literals_to_update: \<open>get_conflict_l_init S = None \<longrightarrow>
+     literals_to_update_l_init S = uminus `# lit_of `# mset (get_trail_l_init S)\<close> and
+    add_inv: \<open>twl_list_invs (fst S)\<close> and
+    stgy_inv: \<open>twl_stgy_invs (fst T)\<close> and
+    OC'_empty: \<open>other_clauses_l_init S \<noteq> {#} \<longrightarrow> get_conflict_l_init S \<noteq> None\<close>
+    using pre unfolding init_dt_pre_def
+    apply -
+    apply normalize_goal+
+    by force
+  obtain M N D NE UE Q U OC where
+    S: \<open>S = ((M, N, U, D, NE, UE, Q), OC)\<close>
+    by (cases S) auto
+  have [simp]: \<open>twl_list_invs (fst (set_conflict_init_l C S))\<close>
+    using add_inv by (auto simp:  set_conflict_init_l_def S
+        twl_list_invs_def)
+  have [simp]: \<open>(set_conflict_init_l C S, set_conflict_init C T)
+        \<in> twl_st_l_init\<close>
+    using SOC_T by (cases S) (auto simp: twl_st_l_init_def set_conflict_init_l_def)
+  have dec': \<open>count_decided (get_trail_init T) = 0\<close>
+    using SOC_T dec SOC_T by (auto simp: twl_st_l_init twl_st_init convert_lits_l_def
+        count_decided_0_iff)
+  have [simp]: \<open>twl_stgy_invs (fst (set_conflict_init C T))\<close>
+    using stgy_inv dec' nempty count_decided_ge_get_level[of \<open>get_trail_init T\<close>]
+    unfolding twl_stgy_invs_def cdcl\<^sub>W_restart_mset.cdcl\<^sub>W_stgy_invariant_def
+       cdcl\<^sub>W_restart_mset.conflict_non_zero_unless_level_0_def cdcl\<^sub>W_restart_mset.no_smaller_confl_def
+    by (cases T; cases C)
+       (auto 5 5 simp: cdcl\<^sub>W_restart_mset_state clauses_def)
+  note clauses_to_update_inv.simps[simp del] valid_enqueued_alt_simps[simp del]
+  have [simp]: \<open>twl_struct_invs_init (set_conflict_init C T)\<close>
+    apply (rule twl_struct_invs_init_set_conflict_init)
+    using inv nempty dist_C SOC_T dec false nempty
+    by (auto simp: twl_st_init count_decided_0_iff)
+  show ?thesis
+    unfolding init_dt_pre_def
+    apply (rule exI[of _ \<open>set_conflict_init C T\<close>])
+    using dist WS dec in_literals_to_update OC'_empty by (auto simp: twl_st_init twl_st_l_init)
+qed
+
+lemma
+  assumes 
+    \<open>get_conflict_l_init S = None\<close> and
+    nempty: \<open>length C = Suc 0\<close> and
+    pre: \<open>init_dt_pre (C # CS) S\<close> and
+    dec: \<open>\<forall>s\<in>set (get_trail_l_init S). \<not> is_decided s\<close> and
+    \<open>hd C \<notin> lits_of_l (get_trail_l_init S)\<close> and
+    \<open>undefined_lit (get_trail_l_init S) (hd C)\<close>
+  shows \<open>init_dt_pre CS (propagate_unit_init_l (hd C) S)\<close>
+proof -
+  obtain T where
+    SOC_T: \<open>(S, T) \<in> twl_st_l_init\<close> and
+    dist: \<open>Ball (set CS) distinct\<close> and
+    dist_C: \<open>distinct C\<close> and
+    inv: \<open>twl_struct_invs_init T\<close> and
+    WS: \<open>clauses_to_update_l_init S = {#}\<close> and
+    dec: \<open>\<forall>s\<in>set (get_trail_l_init S). \<not> is_decided s\<close> and
+    in_literals_to_update: \<open>get_conflict_l_init S = None \<longrightarrow>
+     literals_to_update_l_init S = uminus `# lit_of `# mset (get_trail_l_init S)\<close> and
+    add_inv: \<open>twl_list_invs (fst S)\<close> and
+    stgy_inv: \<open>twl_stgy_invs (fst T)\<close> and
+    OC'_empty: \<open>other_clauses_l_init S \<noteq> {#} \<longrightarrow> get_conflict_l_init S \<noteq> None\<close>
+    using pre unfolding init_dt_pre_def
+    apply -
+    apply normalize_goal+
+    by force
+  let ?L = \<open>hd C\<close>
+  obtain M N D NE UE Q U OC where
+    S: \<open>S = ((M, N, U, D, NE, UE, Q), OC)\<close>
+    by (cases S) auto
+  have [simp]: \<open>twl_list_invs (fst (propagate_unit_init_l ?L S))\<close>
+    using add_inv by (auto simp:  propagate_unit_init_l_def S
+        twl_list_invs_def)
+  have [simp]: \<open>(propagate_unit_init_l ?L S, propagate_unit_init ?L T)
+        \<in> twl_st_l_init\<close>
+    using SOC_T by (cases S) (auto simp: twl_st_l_init_def propagate_unit_init_l_def)
+  have dec': \<open>count_decided (get_trail_init T) = 0\<close>
+    using SOC_T dec SOC_T by (auto simp: twl_st_l_init twl_st_init convert_lits_l_def
+        count_decided_0_iff)
+  have dec': \<open>\<forall>s\<in>set (get_trail_init T). \<not> is_decided s\<close>
+    using SOC_T dec by (auto simp: twl_st_init twl_st_l_init convert_lits_l_def)
+  then have \<open>Propagated (hd C) {#hd C#} # get_trail_init T = M' @ Decided K # M \<longleftrightarrow> False\<close>
+    for M' K M
+    by (cases M') auto
+  then have [simp]: \<open>twl_stgy_invs (fst (propagate_unit_init ?L T))\<close>
+    using stgy_inv dec' nempty count_decided_ge_get_level[of \<open>get_trail_init T\<close>]
+    unfolding twl_stgy_invs_def cdcl\<^sub>W_restart_mset.cdcl\<^sub>W_stgy_invariant_def
+       cdcl\<^sub>W_restart_mset.conflict_non_zero_unless_level_0_def cdcl\<^sub>W_restart_mset.no_smaller_confl_def
+    by (cases T)
+       (auto simp: cdcl\<^sub>W_restart_mset_state clauses_def get_level_cons_if)
+  note clauses_to_update_inv.simps[simp del] valid_enqueued_alt_simps[simp del]
+  have [simp]: \<open>twl_struct_invs_init (propagate_unit_init ?L T)\<close>
+    apply (rule twl_struct_invs_init_set_conflict_init)
+    using inv nempty dist_C SOC_T dec false nempty
+    by (auto simp: twl_st_init count_decided_0_iff)
+  show ?thesis
+    unfolding init_dt_pre_def
+    apply (rule exI[of _ \<open>propagate_unit_init ?L T\<close>])
+    using dist WS dec in_literals_to_update OC'_empty by (auto simp: twl_st_init twl_st_l_init)
+qed
+
+
+lemma
+  assumes pre: \<open>init_dt_pre (a # CS) SOC\<close>
+  shows \<open>init_dt_step a SOC \<le> SPEC (init_dt_pre CS)\<close>
+proof -
+  obtain S OC where SOC: \<open>SOC = (S, OC)\<close>
+    by (cases SOC) auto
+
+  obtain T where
+    SOC_T: \<open>((S, OC), T) \<in> twl_st_l_init\<close> and
+    dist: \<open>Ball (set (a # CS)) distinct\<close> and
+    inv: \<open>twl_struct_invs_init T\<close> and
+    WS: \<open>clauses_to_update_l_init (S, OC) = {#}\<close> and
+    dec: \<open>\<forall>s\<in>set (get_trail_l_init (S, OC)). \<not> is_decided s\<close> and
+    in_literals_to_update: \<open>get_conflict_l_init (S, OC) = None \<longrightarrow>
+     literals_to_update_l_init (S, OC) = uminus `# lit_of `# mset (get_trail_l_init (S, OC))\<close> and
+    add_inv: \<open>twl_list_invs (fst (S, OC))\<close> and
+    stgy_inv: \<open>twl_stgy_invs (fst T)\<close> and
+    OC'_empty: \<open>other_clauses_l_init (S, OC) \<noteq> {#} \<longrightarrow> get_conflict_l_init (S, OC) \<noteq> None\<close>
+    using pre unfolding SOC init_dt_pre_def
+    apply -
+    apply normalize_goal+
+    by presburger
+
+(*   case 2 note dist = this(1) and inv = this(2) and
+    WS = this(3) and dec = this(4) and in_literals_to_update = this(5) and add_inv = this(6) and
+    len = this(7) and stgy_inv = this(8) and OC'_empty = this(9)
+  let ?SOC' = \<open>init_dt CS (S, OC)\<close>
+  let ?S' = \<open>fst (init_dt CS (S, OC))\<close>
+  let ?OC' = \<open>snd (init_dt CS (S, OC))\<close>
+  have
+    twl: \<open>twl_struct_invs_init (twl_st_of_init ?SOC')\<close> and
+    w_q: \<open>clauses_to_update_l ?S' = {#}\<close> and
+    dec': \<open>\<forall>s\<in>set (get_trail_l ?S'). \<not> is_decided s\<close> and
+    literals_to_update': \<open>get_conflict_l ?S' = None \<longrightarrow>
+        literals_to_update_l ?S' = uminus `# lit_of `# mset (get_trail_l ?S')\<close>
+      and
+    clss': \<open>mset `# mset CS + cdcl\<^sub>W_restart_mset.clauses (state\<^sub>W_of (twl_st_of None S)) + OC =
+      cdcl\<^sub>W_restart_mset.clauses (state\<^sub>W_of (twl_st_of None ?S')) + ?OC'\<close>
+      and
+    learned': \<open>learned_clss (state\<^sub>W_of (twl_st_of None ?S')) = learned_clss (state\<^sub>W_of (twl_st_of None S))\<close>
+      and
+    add_inv': \<open>twl_list_invs ?S'\<close> and
+    U': \<open>get_learned_l ?S' = length (get_clauses_l ?S') - 1\<close> and
+    OC'_empty: \<open>snd ?SOC' \<noteq> {#} \<longrightarrow> get_conflict_l ?S' \<noteq> None\<close>and
+    OC'_empty_conflict: \<open>{#} \<in># mset `# mset CS \<longrightarrow> get_conflict_l ?S' \<noteq> None\<close>
+    using IH[OF _ inv WS dec in_literals_to_update add_inv len stgy_inv OC'_empty] dist by auto
+ *)
+  obtain M N D NE UE Q where
+    S: \<open>SOC = ((M, N, D, NE, UE, {#}, Q), OC)\<close>
+    using WS by (cases SOC) (auto simp: SOC)
+  then have S': \<open>S = (M, N, D, NE, UE, {#}, Q)\<close>
+    using S unfolding SOC by auto
+  show ?thesis
+  proof (cases \<open>get_conflict_l (fst SOC)\<close>)
+    case None
+    then show ?thesis
+      apply (auto simp: init_dt_step_def get_fresh_index_def RES_RETURN_RES)
+      using pre dec apply (auto simp add: Let_def count_decided_0_iff SOC twl_st_l_init twl_st_init
+          intro!: init_dt_pre_already_propagated_unit_init_l init_dt_pre_set_conflict_init_l
+          dest: init_dt_pre_ConsD in_lits_of_l_defined_litD)
+      defer
+      explore_lemma
+      sorry
+  next
+    case [simp]: (Some D)
+    have [simp]: \<open>(((M, N, Some D, NE, UE, {#}, Q), add_mset (mset a) OC), add_to_other_init (mset a) T)
+       \<in> twl_st_l_init\<close>
+      \<open>get_trail (fst T) = convert_lits_l N M\<close>
+      using SOC_T by (cases T; auto simp: S S' twl_st_l_init_def; fail)+
+    have \<open>init_dt_pre CS ((M, N, Some D, NE, UE, {#}, Q), add_mset (mset a) OC)\<close>
+      unfolding init_dt_pre_def
+      apply (rule exI[of _ \<open>add_to_other_init (mset a) T\<close>])
+      using dist inv WS dec  in_literals_to_update add_inv stgy_inv SOC_T
+      by (auto simp: S'  count_decided_0_iff
+          intro!: twl_struct_invs_init_add_to_other_init)
+    then show ?thesis
+      by (auto simp: S init_dt_step_def)
+
+  qed
+    apply (auto simp: S init_dt_step_def init_dt_pre_def)
+
+  obtain M N D NE UE Q OCS where
+    S: \<open>init_dt CS (S, OC) = ((M, N, D, NE, UE, {#}, Q), OCS)\<close>
+    using w_q by (cases \<open>init_dt CS (S, OC)\<close>) auto
+  obtain M' N' U' D' NE' WS' UE' Q' where
+    S': \<open>twl_st_of None (fst (init_dt (a # CS) (S, OC))) = (M', N', U', D', NE', UE', WS', Q')\<close>
+    by (cases \<open>twl_st_of None (fst (init_dt (a # CS) (S, OC)))\<close>) auto
+  then have [simp]: \<open>UE' = UE\<close>
+    by (cases a; cases D) (auto simp: S split: if_splits)
+
+  have dec_M: \<open>\<forall>s\<in>set M. \<not> is_decided s\<close>
+    using dec' S by auto
+  have N_not_empty: \<open>N \<noteq> []\<close>
+    using add_inv' unfolding twl_list_invs_def S by auto
+  have U_len_N: \<open>U = length N - 1\<close>
+    using U' unfolding S by auto
+  then have [simp]: \<open>take U (tl N) = tl N\<close> \<open>drop (Suc U) N = []\<close> \<open>drop U (tl N) = []\<close>
+    by auto
+  show ?case using w_q
+    by (cases D) (auto simp: S Let_def)
+  case 3
+  show ?case
+    using dec_M by (cases D) (auto simp: S Let_def)
+  case 4
+  show ?case
+    using literals_to_update' by (cases D) (auto simp: S Let_def)
+  have a_D: \<open>\<exists>x y a'. a = x # y # a'\<close> if \<open>\<forall>L. a \<noteq> [L]\<close> and \<open>a \<noteq> []\<close>
+    apply (case_tac a, (use that in simp; fail))
+    apply (rename_tac aa list, case_tac list; use that in simp)
+    done
+  have mset_tl_N: \<open>{#mset (watched_l x) + mset (unwatched_l x). x \<in># mset (take U (tl N))#} + {#mset (watched_l x) + mset (unwatched_l x). x \<in># mset (drop (Suc U) N)#} =
+         {#mset (watched_l x) + mset (unwatched_l x). x \<in># mset (tl N)#}\<close>
+    unfolding image_mset_union[symmetric] mset_append[symmetric] append_take_drop_id drop_Suc ..
+  case 5
+  show ?case
+    using clss' U_len_N N_not_empty by (cases D)
+      (auto simp: S Let_def clauses_def length_list_Suc_0 cdcl\<^sub>W_restart_mset_state mset_tl_N
+        dest!: a_D)
+  case 6
+  show ?case
+    using learned' U_len_N by (cases D) (auto simp: S Let_def clauses_def length_list_Suc_0
+        cdcl\<^sub>W_restart_mset_state)
+
+  case 7
+  show ?case
+    using add_inv' N_not_empty
+    by (cases D) (fastforce simp add: U_len_N S clauses_def twl_list_invs_def Let_def nth_append
+        cdcl\<^sub>W_restart_mset_state)+
+  case 8
+  show ?case
+    by (cases D) (auto simp add: U_len_N S clauses_def twl_list_invs_def Let_def nth_append
+        cdcl\<^sub>W_restart_mset_state)
+
+  let ?S' = \<open>(convert_lits_l N M, twl_clause_of `# mset (take U (tl N)),
+       twl_clause_of `# mset (drop U (tl N)), D, NE, UE, {#}, Q)\<close>
+  case 1
+  let ?S' = \<open>((convert_lits_l N M, twl_clause_of `# mset (take U (tl N)), twl_clause_of `# mset (drop U (tl N)), D, NE, UE, {#}, Q), OCS)\<close>
+  let ?T' = \<open>state\<^sub>W_of_init ?S'\<close>
+  have
+    struct: \<open>Multiset.Ball (twl_clause_of `# mset (tl N)) struct_wf_twl_cls\<close> and
+    H: \<open>\<forall>C\<in>#twl_clause_of `# mset (tl N). D = None \<longrightarrow>
+      \<not> twl_is_an_exception C Q ({#} :: ('v literal \<times> 'v twl_cls) multiset ) \<longrightarrow>
+      (twl_lazy_update (convert_lits_l N M) C \<and> twl_inv (convert_lits_l N M) C)\<close> and
+    lev: \<open>\<forall>C\<in>#twl_clause_of `# mset (tl N). D = None \<longrightarrow> watched_literals_false_of_max_level (convert_lits_l N M) C\<close> and
+    valid: \<open>valid_enqueued (fst ?S')\<close> and
+    all_struct: \<open>cdcl\<^sub>W_restart_mset.cdcl\<^sub>W_all_struct_inv ?T'\<close> and
+    no_smaller: \<open>cdcl\<^sub>W_restart_mset.no_smaller_propa ?T'\<close> and
+    excep: \<open>twl_st_exception_inv (fst ?S')\<close> and
+    no_dup: \<open>no_duplicate_queued (fst ?S')\<close> and
+    dist_q: \<open>distinct_queued (fst ?S')\<close> and
+    confl_cands: \<open>confl_cands_enqueued (fst ?S')\<close> and
+    propa_cands: \<open>propa_cands_enqueued (fst ?S')\<close> and
+    get_confl: \<open>get_conflict (fst ?S') \<noteq> None \<longrightarrow> clauses_to_update (fst ?S') = {#} \<and>
+    literals_to_update (fst ?S') = {#}\<close> and
+    unit_clss: \<open>entailed_clss_inv (fst ?S')\<close> and
+    w_q: \<open>clauses_to_update_inv (fst ?S')\<close> and
+    past_invs: \<open>past_invs (fst ?S')\<close>
+    using twl unfolding twl_st_inv.simps twl_struct_invs_init_def S twl_st_of.simps
+    image_mset_union[symmetric] mset_append[symmetric] append_take_drop_id drop_Suc S
+    twl_struct_invs_def fst_conv twl_st_of_init.simps by fast+
+
+  have [simp]: \<open>get_level M L = 0\<close> and
+    [simp]: \<open>count_decided M = 0\<close> for L
+    using dec' S by (auto simp: count_decided_0_iff)
+  have nm: \<open>\<forall>s\<in>set (convert_lits_l N M). \<not> is_decided s\<close>
+      using dec_M by (auto simp: convert_lits_l_def)
+  have convert_append_Decided_cons[iff]:
+    \<open>convert_lits_l N M = M'a @ Decided K # Ma \<longleftrightarrow> False\<close>
+    \<open>Propagated L C # convert_lits_l N M = M'a @ Decided K # Ma \<longleftrightarrow> False\<close>
+    for M'a K Ma L C
+    using nm apply fastforce
+    by (metis (no_types, lifting) nm annotated_lit.disc(1)
+          annotated_lit.distinct(1) append_eq_Cons_conv in_set_conv_decomp list_tail_coinc)
+  have
+    alien: \<open>cdcl\<^sub>W_restart_mset.no_strange_atm ?T'\<close> and
+    lev_inv: \<open>cdcl\<^sub>W_restart_mset.cdcl\<^sub>W_M_level_inv ?T'\<close> and
+    learned_tauto: \<open>(\<forall>s\<in>#learned_clss ?T'. \<not> tautology s)\<close> and
+    \<open>cdcl\<^sub>W_restart_mset.distinct_cdcl\<^sub>W_state ?T'\<close> and
+    confl: \<open>cdcl\<^sub>W_restart_mset.cdcl\<^sub>W_conflicting ?T'\<close> and
+    all_decomp: \<open>all_decomposition_implies_m (cdcl\<^sub>W_restart_mset.clauses ?T')
+     (get_all_ann_decomposition (trail ?T'))\<close> and
+    learned: \<open>cdcl\<^sub>W_restart_mset.cdcl\<^sub>W_learned_clause ?T'\<close>
+    using all_struct unfolding cdcl\<^sub>W_restart_mset.cdcl\<^sub>W_all_struct_inv_def S'[symmetric]
+    by fast+
+  have propagated_trail_decomp_iff[iff]: \<open>a @ Propagated La C # b = Propagated L D # M' \<longleftrightarrow>
+        (a = [] \<and> Propagated La C = Propagated L D \<and> b = M') \<or>
+        (a \<noteq> [] \<and> tl a @ Propagated La C # b = M' \<and> hd a = Propagated L D)\<close> for a b La L C D M'
+    by (cases a) auto
+
+  have ex_two_watched_N: \<open>\<exists>L L'. watched_l x = [L, L']\<close> if \<open>x \<in> set (tl N)\<close> for x
+  proof -
+    have \<open>struct_wf_twl_cls (twl_clause_of x)\<close>
+      using struct that by auto
+    then show ?thesis
+      by (cases \<open>twl_clause_of x\<close>) (auto simp: length_list_2 take_2_if)
+  qed
+
+  have in_M_IN_QD: \<open>- La \<in> lits_of_l M \<Longrightarrow> La \<in># Q\<close> if \<open>D = None\<close> for La
+    using S literals_to_update' that by (auto simp: lits_of_def uminus_lit_swap)
+
+  have \<open>x \<in> set M \<Longrightarrow> convert_lit (N @ N') x = convert_lit N x\<close> for x N'
+    using add_inv' by (cases x) (auto simp: nth_append twl_list_invs_def S)
+  then have [simp]: \<open>convert_lits_l (N @ N') M = convert_lits_l N M\<close> for N'
+    unfolding convert_lits_l_def by auto
+  consider
+    (confl) \<open>D \<noteq> None\<close> |
+    (empty) \<open>D = None\<close> and \<open>a = []\<close> |
+    (True) \<open>D = None\<close> and \<open>length a = 1\<close> |
+    (False) \<open>D = None\<close> and \<open>length a \<ge> 2\<close>
+    by (cases a; cases \<open>tl a\<close>) auto
+  then show ?case
+  proof cases
+    case confl
+    then show ?thesis
+      using S' twl dist by (auto simp: S cdcl\<^sub>W_restart_mset_state
+          intro!: twl_struct_invs_init_add_mset)
+  next
+    case a: empty
+    have [simp]: \<open>NE' = NE\<close>
+    using S' by (cases D) (auto simp: a S split: if_splits)
+  note in_M_IN_QD = in_M_IN_QD[OF a(1)]
+  have all_inv':
+    \<open>cdcl\<^sub>W_restart_mset.cdcl\<^sub>W_all_struct_inv (convert_lits_l N M,
+      add_mset {#}
+       ({#mset (watched_l x) + mset (unwatched_l x). x \<in># mset (tl N)#} + NE' + OCS),
+      UE', Some {#})\<close>
+    unfolding cdcl\<^sub>W_restart_mset.cdcl\<^sub>W_all_struct_inv_def S'[symmetric]
+    apply (intro conjI)
+    subgoal
+      using alien by (auto simp: a S cdcl\<^sub>W_restart_mset.no_strange_atm_def cdcl\<^sub>W_restart_mset_state
+          cdcl\<^sub>W_restart_mset.cdcl\<^sub>W_all_struct_inv_def Let_def
+          mset_take_mset_drop_mset atms_of_def
+          dest: in_lits_of_l_defined_litD split: if_splits)
+    subgoal
+      using all_struct by (auto simp: cdcl\<^sub>W_restart_mset.cdcl\<^sub>W_M_level_inv_def cdcl\<^sub>W_restart_mset_state
+          cdcl\<^sub>W_restart_mset.cdcl\<^sub>W_all_struct_inv_def S Let_def split: if_splits)
+    subgoal
+      using all_struct by (auto simp: cdcl\<^sub>W_restart_mset.no_strange_atm_def cdcl\<^sub>W_restart_mset_state
+          cdcl\<^sub>W_restart_mset.cdcl\<^sub>W_all_struct_inv_def S Let_def split: if_splits)
+    subgoal
+      using all_struct by (auto simp: cdcl\<^sub>W_restart_mset_state
+          cdcl\<^sub>W_restart_mset.cdcl\<^sub>W_all_struct_inv_def a S Let_def cdcl\<^sub>W_restart_mset.distinct_cdcl\<^sub>W_state_def
+          split: if_splits)
+    subgoal
+      using confl by (auto simp: a cdcl\<^sub>W_restart_mset.cdcl\<^sub>W_conflicting_def cdcl\<^sub>W_restart_mset_state
+          cdcl\<^sub>W_restart_mset.cdcl\<^sub>W_all_struct_inv_def S Let_def Decided_Propagated_in_iff_in_lits_of_l
+          split: if_splits)
+    subgoal
+      apply (cases \<open>get_all_ann_decomposition (convert_lits_l N M)\<close>)
+      using all_decomp by (auto simp: a cdcl\<^sub>W_restart_mset.no_strange_atm_def cdcl\<^sub>W_restart_mset_state
+          cdcl\<^sub>W_restart_mset.cdcl\<^sub>W_all_struct_inv_def S Let_def clauses_def
+          intro!: all_decomposition_implies_insert_single
+          split: if_splits)
+    subgoal
+      using learned by (auto 5 5 simp: a cdcl\<^sub>W_restart_mset.no_strange_atm_def cdcl\<^sub>W_restart_mset_state
+          cdcl\<^sub>W_restart_mset.cdcl\<^sub>W_all_struct_inv_def S Let_def image_Un
+          cdcl\<^sub>W_restart_mset.cdcl\<^sub>W_learned_clause_def clauses_def
+          split: if_splits)
+    done
+  show ?thesis
+    unfolding twl_struct_invs_init_def S' twl_st_inv.simps
+    apply (intro conjI)
+    subgoal
+      using H S' dec' nm struct by (auto simp: twl_struct_invs_def a S twl_st_inv.simps
+          split: if_splits)
+    subgoal
+      using struct S' by (auto simp: a S split: if_splits)[]
+    subgoal using all_inv' by (auto simp: twl_struct_invs_def a S twl_st_inv.simps
+          split: if_splits)
+    subgoal
+      using S' no_smaller by (auto simp: a S cdcl\<^sub>W_restart_mset_state
+          cdcl\<^sub>W_restart_mset.no_smaller_propa_def clauses_def split: if_splits)
+    subgoal
+      using S' excep by (force simp: a S twl_exception_inv.simps split: if_splits)
+    subgoal
+      using S' by (auto simp: a S split: if_splits)
+    subgoal
+      using S' excep by (force simp: a S twl_exception_inv.simps split: if_splits)
+    subgoal
+      using S' no_dup by (auto simp: a S cdcl\<^sub>W_restart_mset_state
+          twl_exception_inv.simps uminus_lit_swap
+          cdcl\<^sub>W_restart_mset.no_smaller_propa_def clauses_def split: if_splits)
+    subgoal
+      using S' dist_q literals_to_update' by (auto simp add: a S cdcl\<^sub>W_restart_mset_state
+          twl_exception_inv.simps Decided_Propagated_in_iff_in_lits_of_l lits_of_def
+          cdcl\<^sub>W_restart_mset.no_smaller_propa_def clauses_def split: if_splits)
+    subgoal
+      using S' confl_cands by (auto simp: a S cdcl\<^sub>W_restart_mset_state
+          twl_exception_inv.simps uminus_lit_swap true_annots_true_cls_def_iff_negation_in_model
+          cdcl\<^sub>W_restart_mset.no_smaller_propa_def clauses_def conj_disj_distribR ex_disj_distrib
+          dest: in_diffD dest!: in_M_IN_QD dest!: ex_two_watched_N
+          split: if_splits)
+    subgoal
+      using S' propa_cands unit_clss by (auto simp: a S cdcl\<^sub>W_restart_mset_state
+          twl_exception_inv.simps uminus_lit_swap true_annots_true_cls_def_iff_negation_in_model
+          cdcl\<^sub>W_restart_mset.no_smaller_propa_def clauses_def conj_disj_distribR ex_disj_distrib
+          dest: in_diffD dest!: in_M_IN_QD dest!: ex_two_watched_N
+          split: if_splits)
+    subgoal
+      using S' by (auto simp: a S cdcl\<^sub>W_restart_mset_state
+          twl_exception_inv.simps uminus_lit_swap
+          cdcl\<^sub>W_restart_mset.no_smaller_propa_def clauses_def split: if_splits)
+    subgoal
+      using S' past_invs by (auto simp: a S past_invs.simps
+          cdcl\<^sub>W_restart_mset.no_smaller_propa_def clauses_def split: if_splits)
+    done
+  next
+    case True note _[simp] = this(1) and a = this(2)
+    then obtain L where a: \<open>a = [L]\<close>
+      using list_decomp_1 by blast
+    note in_M_IN_QD = in_M_IN_QD[OF True(1)]
+    have all_inv':
+      \<open>cdcl\<^sub>W_restart_mset.cdcl\<^sub>W_all_struct_inv (state\<^sub>W_of_init (twl_st_of_init (init_dt (a # CS) (S, OC))))\<close>
+      unfolding cdcl\<^sub>W_restart_mset.cdcl\<^sub>W_all_struct_inv_def S'[symmetric]
+        init_dt.simps S
+      apply (intro conjI)
+      subgoal
+        using alien by (auto simp: a S cdcl\<^sub>W_restart_mset.no_strange_atm_def cdcl\<^sub>W_restart_mset_state
+            cdcl\<^sub>W_restart_mset.cdcl\<^sub>W_all_struct_inv_def Let_def dest: in_lits_of_l_defined_litD split: if_splits)
+      subgoal
+        using all_struct by (auto simp: cdcl\<^sub>W_restart_mset.cdcl\<^sub>W_M_level_inv_def cdcl\<^sub>W_restart_mset_state
+            cdcl\<^sub>W_restart_mset.cdcl\<^sub>W_all_struct_inv_def S Let_def split: if_splits)
+      subgoal
+        using all_struct by (auto simp: cdcl\<^sub>W_restart_mset.no_strange_atm_def cdcl\<^sub>W_restart_mset_state
+            cdcl\<^sub>W_restart_mset.cdcl\<^sub>W_all_struct_inv_def S Let_def split: if_splits)
+      subgoal
+        using all_struct by (auto simp: cdcl\<^sub>W_restart_mset_state
+            cdcl\<^sub>W_restart_mset.cdcl\<^sub>W_all_struct_inv_def a S Let_def cdcl\<^sub>W_restart_mset.distinct_cdcl\<^sub>W_state_def
+            split: if_splits)
+      subgoal
+        using confl by (auto simp: a cdcl\<^sub>W_restart_mset.cdcl\<^sub>W_conflicting_def cdcl\<^sub>W_restart_mset_state
+            cdcl\<^sub>W_restart_mset.cdcl\<^sub>W_all_struct_inv_def S Let_def Decided_Propagated_in_iff_in_lits_of_l
+            split: if_splits)
+      subgoal
+        apply (cases \<open>get_all_ann_decomposition (convert_lits_l N M)\<close>)
+        using all_decomp by (auto simp: a cdcl\<^sub>W_restart_mset.no_strange_atm_def cdcl\<^sub>W_restart_mset_state
+            cdcl\<^sub>W_restart_mset.cdcl\<^sub>W_all_struct_inv_def S Let_def clauses_def
+            intro!: all_decomposition_implies_insert_single
+            split: if_splits)
+      subgoal
+        using learned by (auto simp: a cdcl\<^sub>W_restart_mset.no_strange_atm_def cdcl\<^sub>W_restart_mset_state
+            cdcl\<^sub>W_restart_mset.cdcl\<^sub>W_all_struct_inv_def S Let_def
+            cdcl\<^sub>W_restart_mset.cdcl\<^sub>W_learned_clause_def clauses_def
+            split: if_splits)
+      done
+    show ?thesis
+      unfolding twl_struct_invs_init_def S' twl_st_inv.simps
+      apply (intro conjI)
+      subgoal
+        using H S' dec' nm struct by (auto simp: twl_struct_invs_def a S twl_st_inv.simps
+            split: if_splits)
+      subgoal
+        using H S' valid by (auto simp: twl_struct_invs_def a S twl_st_inv.simps
+            get_level_cons_if split: if_splits)
+      subgoal using all_inv'
+        using S' by (auto simp: a S cdcl\<^sub>W_restart_mset_state
+            twl_exception_inv.simps uminus_lit_swap
+            cdcl\<^sub>W_restart_mset.no_smaller_propa_def clauses_def split: if_splits)
+      subgoal
+        using S' no_smaller by (auto simp: a S cdcl\<^sub>W_restart_mset_state
+            cdcl\<^sub>W_restart_mset.no_smaller_propa_def clauses_def split: if_splits)
+      subgoal
+        using S' excep by (force simp: a S twl_exception_inv.simps split: if_splits)
+      subgoal
+        using S' no_dup by (auto simp: a S cdcl\<^sub>W_restart_mset_state
+            twl_exception_inv.simps uminus_lit_swap
+            cdcl\<^sub>W_restart_mset.no_smaller_propa_def clauses_def split: if_splits)
+      subgoal
+        using S' dist_q literals_to_update' by (auto simp add: a S cdcl\<^sub>W_restart_mset_state
+            twl_exception_inv.simps Decided_Propagated_in_iff_in_lits_of_l lits_of_def
+            cdcl\<^sub>W_restart_mset.no_smaller_propa_def clauses_def split: if_splits)
+      subgoal
+        using S' confl_cands by (auto simp: a S cdcl\<^sub>W_restart_mset_state
+            twl_exception_inv.simps uminus_lit_swap true_annots_true_cls_def_iff_negation_in_model
+            cdcl\<^sub>W_restart_mset.no_smaller_propa_def clauses_def conj_disj_distribR ex_disj_distrib
+            dest: in_diffD dest!: in_M_IN_QD dest!: ex_two_watched_N
+            split: if_splits)
+      subgoal
+        using S' propa_cands by (auto simp: a S cdcl\<^sub>W_restart_mset_state
+            twl_exception_inv.simps uminus_lit_swap true_annots_true_cls_def_iff_negation_in_model
+            cdcl\<^sub>W_restart_mset.no_smaller_propa_def clauses_def conj_disj_distribR ex_disj_distrib
+            dest: in_diffD dest!: in_M_IN_QD dest!: ex_two_watched_N
+            split: if_splits)
+      subgoal
+        using struct S' by (auto simp: a S split: if_splits)[]
+      subgoal
+        using S' unit_clss by (auto 3 3 simp: a S cdcl\<^sub>W_restart_mset_state
+            twl_exception_inv.simps uminus_lit_swap get_level_cons_if
+            cdcl\<^sub>W_restart_mset.no_smaller_propa_def clauses_def split: if_splits)
+      subgoal
+        using S' w_q by (auto simp: a S cdcl\<^sub>W_restart_mset_state
+            twl_exception_inv.simps uminus_lit_swap get_level_cons_if filter_mset_empty_conv
+            clauses_to_update_prop.simps
+            cdcl\<^sub>W_restart_mset.no_smaller_propa_def clauses_def split: if_splits
+            dest: in_M_IN_QD)
+      subgoal
+        using S' past_invs by (auto simp: a S past_invs.simps
+            cdcl\<^sub>W_restart_mset.no_smaller_propa_def clauses_def split: if_splits)
+      done
+  next
+    case False note [simp] = this(1) and a = this(2)
+    then have [simp]: \<open>length a \<noteq> Suc 0\<close> by auto
+    then obtain x y a' where a: \<open>a = x # y # a'\<close>
+      apply (case_tac a, (use False in simp; fail))
+      apply (rename_tac aa list, case_tac list; simp)
+      done
+    have all_inv':
+      \<open>cdcl\<^sub>W_restart_mset.cdcl\<^sub>W_all_struct_inv (state\<^sub>W_of_init (twl_st_of_init (init_dt (a # CS) (S, OC))))\<close>
+      unfolding cdcl\<^sub>W_restart_mset.cdcl\<^sub>W_all_struct_inv_def S'[symmetric]
+      apply (intro conjI)
+      subgoal
+        using alien N_not_empty
+        by (auto 3 3 simp: a S cdcl\<^sub>W_restart_mset.no_strange_atm_def cdcl\<^sub>W_restart_mset_state
+            cdcl\<^sub>W_restart_mset.cdcl\<^sub>W_all_struct_inv_def Let_def dest: (* in_lits_of_l_defined_litD *)
+            split: if_splits)
+      subgoal
+        using all_struct by (auto simp: cdcl\<^sub>W_restart_mset.cdcl\<^sub>W_M_level_inv_def cdcl\<^sub>W_restart_mset_state
+            cdcl\<^sub>W_restart_mset.cdcl\<^sub>W_all_struct_inv_def S Let_def split: if_splits)
+      subgoal
+        using all_struct by (auto simp: cdcl\<^sub>W_restart_mset.no_strange_atm_def cdcl\<^sub>W_restart_mset_state
+            cdcl\<^sub>W_restart_mset.cdcl\<^sub>W_all_struct_inv_def S Let_def split: if_splits)
+      subgoal
+        using all_struct dist N_not_empty by (auto simp: cdcl\<^sub>W_restart_mset_state
+            cdcl\<^sub>W_restart_mset.cdcl\<^sub>W_all_struct_inv_def a S Let_def cdcl\<^sub>W_restart_mset.distinct_cdcl\<^sub>W_state_def
+            convert_lits_l_append split: if_splits)
+      subgoal
+        using confl by (auto simp: a cdcl\<^sub>W_restart_mset.cdcl\<^sub>W_conflicting_def cdcl\<^sub>W_restart_mset_state
+            cdcl\<^sub>W_restart_mset.cdcl\<^sub>W_all_struct_inv_def S Let_def propagated_trail_decomp_iff
+            Decided_Propagated_in_iff_in_lits_of_l
+            split: if_splits)
+      subgoal
+        apply (cases \<open>get_all_ann_decomposition (convert_lits_l N M)\<close>)
+        using all_decomp N_not_empty by (auto simp: a cdcl\<^sub>W_restart_mset.no_strange_atm_def cdcl\<^sub>W_restart_mset_state
+            cdcl\<^sub>W_restart_mset.cdcl\<^sub>W_all_struct_inv_def S Let_def clauses_def
+            intro!: all_decomposition_implies_insert_single
+            split: if_splits)
+      subgoal
+        using learned N_not_empty by (auto simp: a cdcl\<^sub>W_restart_mset.no_strange_atm_def cdcl\<^sub>W_restart_mset_state
+            cdcl\<^sub>W_restart_mset.cdcl\<^sub>W_all_struct_inv_def S Let_def
+            cdcl\<^sub>W_restart_mset.cdcl\<^sub>W_learned_clause_def clauses_def
+            split: if_splits)
+      done
+    show ?thesis
+      unfolding twl_struct_invs_init_def S' twl_st_inv.simps
+      apply (intro conjI)
+      subgoal
+        using H S' dec struct N_not_empty dist by (auto simp: twl_struct_invs_def a S twl_st_inv.simps
+            split: if_splits)
+      subgoal
+        using H S' valid by (auto simp: twl_struct_invs_def a S twl_st_inv.simps
+            get_level_cons_if
+            split: if_splits)
+      subgoal using all_inv' .
+      subgoal
+        using S' no_smaller by (auto simp: a S cdcl\<^sub>W_restart_mset_state
+            cdcl\<^sub>W_restart_mset.no_smaller_propa_def clauses_def split: if_splits)
+      subgoal
+        using S' excep in_M_IN_QD by (auto simp: a S cdcl\<^sub>W_restart_mset_state
+            twl_exception_inv.simps uminus_lit_swap add_mset_eq_add_mset
+            cdcl\<^sub>W_restart_mset.no_smaller_propa_def clauses_def
+            split: if_splits)
+      subgoal
+        using S' no_dup by (auto simp: a S cdcl\<^sub>W_restart_mset_state
+            twl_exception_inv.simps uminus_lit_swap
+            cdcl\<^sub>W_restart_mset.no_smaller_propa_def clauses_def split: if_splits)
+      subgoal
+        using S' dist_q in_literals_to_update by (auto simp add: a S cdcl\<^sub>W_restart_mset_state
+            twl_exception_inv.simps Decided_Propagated_in_iff_in_lits_of_l lits_of_def
+            cdcl\<^sub>W_restart_mset.no_smaller_propa_def clauses_def split: if_splits)
+      subgoal
+        using S' confl_cands in_M_IN_QD N_not_empty by (force simp: a S cdcl\<^sub>W_restart_mset_state
+            twl_exception_inv.simps uminus_lit_swap ex_disj_distrib conj_disj_distribR
+            cdcl\<^sub>W_restart_mset.no_smaller_propa_def clauses_def
+            dest!: in_M_IN_QD dest!: ex_two_watched_N
+            split: if_splits)+
+      subgoal
+        using S' propa_cands in_M_IN_QD N_not_empty by (auto simp: a S cdcl\<^sub>W_restart_mset_state
+            twl_exception_inv.simps uminus_lit_swap ex_disj_distrib conj_disj_distribR
+            all_conj_distrib cdcl\<^sub>W_restart_mset.no_smaller_propa_def clauses_def
+            dest!: ex_two_watched_N split: if_splits)
+      subgoal by (auto simp: S Let_def a split: if_splits)
+
+      subgoal
+        using S' unit_clss by (cases D) (auto simp: a S cdcl\<^sub>W_restart_mset_state
+            twl_exception_inv.simps uminus_lit_swap get_level_cons_if
+            cdcl\<^sub>W_restart_mset.no_smaller_propa_def clauses_def split: if_splits)
+      subgoal
+        using S' w_q in_M_IN_QD by (cases D) (auto simp: a S cdcl\<^sub>W_restart_mset_state
+            twl_exception_inv.simps uminus_lit_swap get_level_cons_if filter_mset_empty_conv
+            clauses_to_update_prop.simps
+            cdcl\<^sub>W_restart_mset.no_smaller_propa_def clauses_def
+            split: if_splits)
+      subgoal
+        apply (cases D)
+        using S' past_invs by (auto simp: a S past_invs.simps
+            cdcl\<^sub>W_restart_mset.no_smaller_propa_def clauses_def split: if_splits)
+      done
+  qed
+  case 9
+  show ?case
+    unfolding twl_stgy_invs_def cdcl\<^sub>W_restart_mset.cdcl\<^sub>W_stgy_invariant_def
+       cdcl\<^sub>W_restart_mset.conflict_non_zero_unless_level_0_def
+    by (cases D; cases a)
+        (auto simp: S cdcl\<^sub>W_restart_mset.no_smaller_confl_def clauses_def
+        cdcl\<^sub>W_restart_mset_state Let_def)
+
+  case 10
+  show ?case
+    using OC'_empty
+    by (cases D; cases a) (auto simp: S cdcl\<^sub>W_restart_mset_state Let_def)
+  case 11
+  show ?case
+    using OC'_empty_conflict
+    by (cases D; cases a) (auto simp: S cdcl\<^sub>W_restart_mset_state Let_def)
+qed
+
+lemma init_dt_full:
+  fixes CS :: \<open>'v literal list list\<close> and SOC :: \<open>'v twl_st_l_init\<close> and S'
+(*   defines \<open>SOC' \<equiv> init_dt CS (S, OC)\<close>
+  defines \<open>S' \<equiv> fst (init_dt CS (S, OC))\<close>
+  defines \<open>OC' \<equiv> snd (init_dt CS (S, OC))\<close> *)
+  defines
+    \<open>S \<equiv> fst SOC\<close> and
+    \<open>OC \<equiv> snd SOC\<close>
+  assumes
+    \<open>init_dt_pre CS SOC\<close>
+  shows
+    \<open>init_dt CS SOC \<le> SPEC (init_dt_spec CS SOC)\<close>
+(*     \<open>twl_struct_invs_init (twl_st_of_init SOC')\<close> and
     \<open>clauses_to_update_l S' = {#}\<close> and
     \<open>\<forall>s\<in>set (get_trail_l S'). \<not>is_decided s\<close> and
     \<open>get_conflict_l S' = None \<longrightarrow> literals_to_update_l S' = uminus `# lit_of `# mset (get_trail_l S')\<close> and
@@ -140,10 +1223,56 @@ lemma init_dt_full:
     \<open>get_learned_l S' = length (get_clauses_l S') - 1\<close> and
     \<open>twl_stgy_invs (twl_st_of None S')\<close> and
     \<open>OC' \<noteq> {#} \<longrightarrow> get_conflict_l S' \<noteq> None\<close> and
-    \<open>{#} \<in># mset `# mset CS \<longrightarrow> get_conflict_l S' \<noteq> None\<close>
-  using assms unfolding S'_def OC'_def SOC'_def OC'_def
-proof (induction CS)
+    \<open>{#} \<in># mset `# mset CS \<longrightarrow> get_conflict_l S' \<noteq> None\<close> *)
+  using assms unfolding S_def OC_def
+proof (induction CS arbitrary: SOC)
   case Nil
+  then obtain S OC where SOC: \<open>SOC = (S, OC)\<close>
+    by (cases SOC) auto
+  from Nil
+  obtain T where
+    T: \<open>(SOC, T) \<in> twl_st_l_init\<close>
+      \<open>Ball (set []) distinct\<close> 
+      \<open>twl_struct_invs_init T\<close> 
+      \<open>clauses_to_update_l (fst SOC) = {#}\<close> 
+      \<open>\<forall>s\<in>set (get_trail_l (fst SOC)). \<not> is_decided s\<close> 
+      \<open>get_conflict_l (fst SOC) = None \<longrightarrow>
+       literals_to_update_l (fst SOC) =
+       uminus `# lit_of `# mset (get_trail_l (fst SOC))\<close> 
+      \<open>twl_list_invs (fst SOC)\<close> 
+      \<open>twl_stgy_invs (fst T)\<close> 
+      \<open>snd SOC \<noteq> {#} \<longrightarrow> get_conflict_l (fst SOC) \<noteq> None\<close>
+    unfolding init_dt_pre_def apply -
+    apply normalize_goal+
+    by auto
+
+  show ?case
+    unfolding init_dt.simps SOC init_dt_spec_def
+    apply (intro RETURN_rule)
+    unfolding prod.simps
+    apply (rule exI[of _ T])
+    using T by (auto simp: SOC)
+next
+  case (Cons a CS) note IH = this(1) and pre = this(2)
+  note init_dt_step_def[simp]
+  have 1: \<open>init_dt_step a SOC \<le> SPEC (init_dt_pre CS)\<close> if  \<open>init_dt_pre (a # CS) SOC\<close>
+    unfolding init_dt_pre_def
+    apply (cases SOC)
+    apply (auto)
+    sorry
+  show ?case
+    unfolding init_dt.simps
+    apply (rule specify_left)
+     apply (rule 1)
+    apply (rule order.trans)
+     apply (rule IH)
+    apply assumption
+    thm IH
+
+
+    oops
+
+
   case 1 then show ?case by simp
   case 2 then show ?case by simp
   case 3 then show ?case by simp
