Weidenbach_Book/Watched_Literals_Watch_List.thy
@@ -1287,12 +1287,6 @@ fun equality_except_trail_wl :: \<open>'v twl_st_wl \<Rightarrow> 'v twl_st_wl \
 \<open>equality_except_trail_wl (M, N, D, NE, UE, WS, Q) (M', N', D', NE', UE', WS', Q') \<longleftrightarrow>
     N = N' \<and> D = D' \<and> NE = NE' \<and> UE = UE' \<and> WS = WS' \<and> Q = Q'\<close>
 
-method normalize_goal =
-  (match premises in
-    J[thin]: \<open>\<exists>x. _\<close> \<Rightarrow> \<open>rule exE[OF J]\<close>
-  \<bar> J[thin]: \<open>_ \<and> _\<close> \<Rightarrow> \<open>rule conjE[OF J]\<close>
-  )
-
 lemma backtrack_wl_spec:
   \<open>(backtrack_wl, backtrack_l)
     \<in> {(T'::'v twl_st_wl, T).
